PO -> Ord, wPO -> wOrd

CAT/SO.v
@@ -22,9 +22,9 @@ Program Instance wPO_struct : Cat_struct (fun a b : PO_obj => a -> b) := {
    comp a b c := fun (f:a -> b) (g:b -> c) => fun x => g (f x)
 }.
 
-Definition wPO := Build_Cat wPO_struct.
+Definition wOrd := Build_Cat wPO_struct.
 
-Class Monotone (a b : wPO) (f : a ---> b) := 
+Class Monotone (a b : wOrd) (f : a ---> b) := 
   monotone : Proper (Rel ==> Rel) f.
 
 Obligation Tactic := mauto ; unfold Monotone; cat;
@@ -32,19 +32,19 @@ Obligation Tactic := mauto ; unfold Monotone; cat;
 (*
 Obligation Tactic := idtac.
 *)
-Program Instance wPO_monotone_SubCat : SubCat_compat wPO
+Program Instance wPO_monotone_SubCat : SubCat_compat wOrd
       (fun x => True) (fun a b f => Monotone f).
 
 Definition wPO_monotone := SubCat wPO_monotone_SubCat.
 
-Program Instance wPO_prod : Cat_Prod (wPO) := {
+Program Instance wPO_prod : Cat_Prod wOrd := {
   product a b := PO_product a b;
   prl a b := fst;
   prr a b := snd;
   prod_mor a b c f g := fun z => (f z, g z)
 }.
 
-Program Instance wPO_Terminal : Terminal wPO := {
+Program Instance wPO_Terminal : Terminal wOrd := {
   Term := PO_TERM;
   TermMor a := fun x => tt
 }.
@@ -53,7 +53,7 @@ Obligation Tactic := simpl; intros;
   repeat match goal with [H:TEMPTY |- _ ] => elim H end;
       cat.
 
-Program Instance TYPE_init : Initial wPO := {
+Program Instance TYPE_init : Initial wOrd := {
   Init := PO_INIT 
 }.
 
